pulse/lib/steel/pulse/Pulse.Typing.Combinators.fsti
@@ -80,25 +80,6 @@ type st_typing_in_ctxt (g:env) (ctxt:vprop) (post_hint:post_hint_opt g) =
   c:comp { stateful_comp c ==> (comp_pre c == ctxt /\ comp_post_matches_hint c post_hint) } &
   st_typing g t c
 
-let x_t_ctxt_match_post_hint
-  (g:env)
-  (post_hint:post_hint_opt g)
-  (x:var) (t:term) (ctxt:vprop) =
-
-  match post_hint with
-  | None -> True
-  | Some post_hint ->
-    t == post_hint.ret_ty /\
-    ctxt == open_term post_hint.post x
- 
-val return_in_ctxt (g:env) (y:var) (u:universe) (ty:term) (ctxt:vprop)
-  (ty_typing:universe_of g ty u)
-  (post_hint0:post_hint_opt g { Some? post_hint0 /\ x_t_ctxt_match_post_hint g post_hint0 y ty ctxt})
-
-  : Pure (st_typing_in_ctxt g ctxt post_hint0)
-         (requires lookup g y == Some ty)
-         (ensures fun _ -> True)
-
 let rec vprop_as_list (vp:term)
   : list term
   = match vp.t with
